feat(DynamoDbEncryption): Add GetEncryptedDataKeyDescription operation (#856)

DynamoDbEncryption/runtimes/java/src/main/smithy-generated/software/amazon/cryptography/dbencryptionsdk/dynamodb/ToNative.java
@@ -30,9 +30,13 @@ import software.amazon.cryptography.dbencryptionsdk.dynamodb.model.DynamoDbEncry
 import software.amazon.cryptography.dbencryptionsdk.dynamodb.model.DynamoDbEncryptionException;
 import software.amazon.cryptography.dbencryptionsdk.dynamodb.model.DynamoDbTableEncryptionConfig;
 import software.amazon.cryptography.dbencryptionsdk.dynamodb.model.DynamoDbTablesEncryptionConfig;
+import software.amazon.cryptography.dbencryptionsdk.dynamodb.model.EncryptedDataKeyDescription;
 import software.amazon.cryptography.dbencryptionsdk.dynamodb.model.EncryptedPart;
 import software.amazon.cryptography.dbencryptionsdk.dynamodb.model.GetBranchKeyIdFromDdbKeyInput;
 import software.amazon.cryptography.dbencryptionsdk.dynamodb.model.GetBranchKeyIdFromDdbKeyOutput;
+import software.amazon.cryptography.dbencryptionsdk.dynamodb.model.GetEncryptedDataKeyDescriptionInput;
+import software.amazon.cryptography.dbencryptionsdk.dynamodb.model.GetEncryptedDataKeyDescriptionOutput;
+import software.amazon.cryptography.dbencryptionsdk.dynamodb.model.GetEncryptedDataKeyDescriptionUnion;
 import software.amazon.cryptography.dbencryptionsdk.dynamodb.model.GetPrefix;
 import software.amazon.cryptography.dbencryptionsdk.dynamodb.model.GetSegment;
 import software.amazon.cryptography.dbencryptionsdk.dynamodb.model.GetSegments;
@@ -360,6 +364,40 @@ public class ToNative {
     return nativeBuilder.build();
   }
 
+  public static EncryptedDataKeyDescription EncryptedDataKeyDescription(
+    software.amazon.cryptography.dbencryptionsdk.dynamodb.internaldafny.types.EncryptedDataKeyDescription dafnyValue
+  ) {
+    EncryptedDataKeyDescription.Builder nativeBuilder =
+      EncryptedDataKeyDescription.builder();
+    nativeBuilder.keyProviderId(
+      software.amazon.smithy.dafny.conversion.ToNative.Simple.String(
+        dafnyValue.dtor_keyProviderId()
+      )
+    );
+    if (dafnyValue.dtor_keyProviderInfo().is_Some()) {
+      nativeBuilder.keyProviderInfo(
+        software.amazon.smithy.dafny.conversion.ToNative.Simple.String(
+          dafnyValue.dtor_keyProviderInfo().dtor_value()
+        )
+      );
+    }
+    if (dafnyValue.dtor_branchKeyId().is_Some()) {
+      nativeBuilder.branchKeyId(
+        software.amazon.smithy.dafny.conversion.ToNative.Simple.String(
+          dafnyValue.dtor_branchKeyId().dtor_value()
+        )
+      );
+    }
+    if (dafnyValue.dtor_branchKeyVersion().is_Some()) {
+      nativeBuilder.branchKeyVersion(
+        software.amazon.smithy.dafny.conversion.ToNative.Simple.String(
+          dafnyValue.dtor_branchKeyVersion().dtor_value()
+        )
+      );
+    }
+    return nativeBuilder.build();
+  }
+
   public static EncryptedPart EncryptedPart(
     software.amazon.cryptography.dbencryptionsdk.dynamodb.internaldafny.types.EncryptedPart dafnyValue
   ) {
@@ -398,6 +436,30 @@ public class ToNative {
     nativeBuilder.branchKeyId(
       software.amazon.smithy.dafny.conversion.ToNative.Simple.String(
         dafnyValue.dtor_branchKeyId()
+      )
+    );
+    return nativeBuilder.build();
+  }
+
+  public static GetEncryptedDataKeyDescriptionInput GetEncryptedDataKeyDescriptionInput(
+    software.amazon.cryptography.dbencryptionsdk.dynamodb.internaldafny.types.GetEncryptedDataKeyDescriptionInput dafnyValue
+  ) {
+    GetEncryptedDataKeyDescriptionInput.Builder nativeBuilder =
+      GetEncryptedDataKeyDescriptionInput.builder();
+    nativeBuilder.input(
+      ToNative.GetEncryptedDataKeyDescriptionUnion(dafnyValue.dtor_input())
+    );
+    return nativeBuilder.build();
+  }
+
+  public static GetEncryptedDataKeyDescriptionOutput GetEncryptedDataKeyDescriptionOutput(
+    software.amazon.cryptography.dbencryptionsdk.dynamodb.internaldafny.types.GetEncryptedDataKeyDescriptionOutput dafnyValue
+  ) {
+    GetEncryptedDataKeyDescriptionOutput.Builder nativeBuilder =
+      GetEncryptedDataKeyDescriptionOutput.builder();
+    nativeBuilder.EncryptedDataKeyDescriptionOutput(
+      ToNative.EncryptedDataKeyDescriptionList(
+        dafnyValue.dtor_EncryptedDataKeyDescriptionOutput()
       )
     );
     return nativeBuilder.build();
@@ -724,6 +786,28 @@ public class ToNative {
     return nativeBuilder.build();
   }
 
+  public static GetEncryptedDataKeyDescriptionUnion GetEncryptedDataKeyDescriptionUnion(
+    software.amazon.cryptography.dbencryptionsdk.dynamodb.internaldafny.types.GetEncryptedDataKeyDescriptionUnion dafnyValue
+  ) {
+    GetEncryptedDataKeyDescriptionUnion.Builder nativeBuilder =
+      GetEncryptedDataKeyDescriptionUnion.builder();
+    if (dafnyValue.is_header()) {
+      nativeBuilder.header(
+        software.amazon.smithy.dafny.conversion.ToNative.Simple.ByteBuffer(
+          dafnyValue.dtor_header()
+        )
+      );
+    }
+    if (dafnyValue.is_item()) {
+      nativeBuilder.item(
+        software.amazon.cryptography.services.dynamodb.internaldafny.ToNative.AttributeMap(
+          dafnyValue.dtor_item()
+        )
+      );
+    }
+    return nativeBuilder.build();
+  }
+
   public static VirtualTransform VirtualTransform(
     software.amazon.cryptography.dbencryptionsdk.dynamodb.internaldafny.types.VirtualTransform dafnyValue
   ) {
@@ -798,6 +882,19 @@ public class ToNative {
     return software.amazon.smithy.dafny.conversion.ToNative.Aggregate.GenericToList(
       dafnyValue,
       software.amazon.cryptography.dbencryptionsdk.dynamodb.ToNative::ConstructorPart
+    );
+  }
+
+  public static List<
+    EncryptedDataKeyDescription
+  > EncryptedDataKeyDescriptionList(
+    DafnySequence<
+      ? extends software.amazon.cryptography.dbencryptionsdk.dynamodb.internaldafny.types.EncryptedDataKeyDescription
+    > dafnyValue
+  ) {
+    return software.amazon.smithy.dafny.conversion.ToNative.Aggregate.GenericToList(
+      dafnyValue,
+      software.amazon.cryptography.dbencryptionsdk.dynamodb.ToNative::EncryptedDataKeyDescription
     );
   }
 
