DynamoDbEncryption/runtimes/java/src/main/smithy-generated/software/amazon/cryptography/dbencryptionsdk/dynamodb/model/GetEncryptedDataKeyDescriptionInput.java
@@ -1,0 +1,67 @@
+// Copyright Amazon.com Inc. or its affiliates. All Rights Reserved.
+// SPDX-License-Identifier: Apache-2.0
+// Do not modify this file. This file is machine generated, and any changes to it will be overwritten.
+package software.amazon.cryptography.dbencryptionsdk.dynamodb.model;
+
+import java.util.Objects;
+
+/**
+ * Input for getting encrypted data key description.
+ */
+public class GetEncryptedDataKeyDescriptionInput {
+
+  private final GetEncryptedDataKeyDescriptionUnion input;
+
+  protected GetEncryptedDataKeyDescriptionInput(BuilderImpl builder) {
+    this.input = builder.input();
+  }
+
+  public GetEncryptedDataKeyDescriptionUnion input() {
+    return this.input;
+  }
+
+  public Builder toBuilder() {
+    return new BuilderImpl(this);
+  }
+
+  public static Builder builder() {
+    return new BuilderImpl();
+  }
+
+  public interface Builder {
+    Builder input(GetEncryptedDataKeyDescriptionUnion input);
+
+    GetEncryptedDataKeyDescriptionUnion input();
+
+    GetEncryptedDataKeyDescriptionInput build();
+  }
+
+  static class BuilderImpl implements Builder {
+
+    protected GetEncryptedDataKeyDescriptionUnion input;
+
+    protected BuilderImpl() {}
+
+    protected BuilderImpl(GetEncryptedDataKeyDescriptionInput model) {
+      this.input = model.input();
+    }
+
+    public Builder input(GetEncryptedDataKeyDescriptionUnion input) {
+      this.input = input;
+      return this;
+    }
+
+    public GetEncryptedDataKeyDescriptionUnion input() {
+      return this.input;
+    }
+
+    public GetEncryptedDataKeyDescriptionInput build() {
+      if (Objects.isNull(this.input())) {
+        throw new IllegalArgumentException(
+          "Missing value for required field `input`"
+        );
+      }
+      return new GetEncryptedDataKeyDescriptionInput(this);
+    }
+  }
+}
