DynamoDbEncryption/runtimes/net/Generated/DynamoDbEncryption/TypeConversion.cs
@@ -179,6 +179,53 @@ namespace AWS.Cryptography.DbEncryptionSDK.DynamoDb
 
       return new software.amazon.cryptography.dbencryptionsdk.dynamodb.internaldafny.types.GetBranchKeyIdFromDdbKeyOutput(ToDafny_N3_aws__N12_cryptography__N15_dbEncryptionSdk__N8_dynamoDb__S30_GetBranchKeyIdFromDdbKeyOutput__M11_branchKeyId(value.BranchKeyId));
     }
+    public static AWS.Cryptography.DbEncryptionSDK.DynamoDb.GetEncryptedDataKeyDescriptionInput FromDafny_N3_aws__N12_cryptography__N15_dbEncryptionSdk__N8_dynamoDb__S35_GetEncryptedDataKeyDescriptionInput(software.amazon.cryptography.dbencryptionsdk.dynamodb.internaldafny.types._IGetEncryptedDataKeyDescriptionInput value)
+    {
+      software.amazon.cryptography.dbencryptionsdk.dynamodb.internaldafny.types.GetEncryptedDataKeyDescriptionInput concrete = (software.amazon.cryptography.dbencryptionsdk.dynamodb.internaldafny.types.GetEncryptedDataKeyDescriptionInput)value; AWS.Cryptography.DbEncryptionSDK.DynamoDb.GetEncryptedDataKeyDescriptionInput converted = new AWS.Cryptography.DbEncryptionSDK.DynamoDb.GetEncryptedDataKeyDescriptionInput(); converted.Input = (AWS.Cryptography.DbEncryptionSDK.DynamoDb.GetEncryptedDataKeyDescriptionUnion)FromDafny_N3_aws__N12_cryptography__N15_dbEncryptionSdk__N8_dynamoDb__S35_GetEncryptedDataKeyDescriptionInput__M5_input(concrete._input); return converted;
+    }
+    public static software.amazon.cryptography.dbencryptionsdk.dynamodb.internaldafny.types._IGetEncryptedDataKeyDescriptionInput ToDafny_N3_aws__N12_cryptography__N15_dbEncryptionSdk__N8_dynamoDb__S35_GetEncryptedDataKeyDescriptionInput(AWS.Cryptography.DbEncryptionSDK.DynamoDb.GetEncryptedDataKeyDescriptionInput value)
+    {
+      value.Validate();
+
+      return new software.amazon.cryptography.dbencryptionsdk.dynamodb.internaldafny.types.GetEncryptedDataKeyDescriptionInput(ToDafny_N3_aws__N12_cryptography__N15_dbEncryptionSdk__N8_dynamoDb__S35_GetEncryptedDataKeyDescriptionInput__M5_input(value.Input));
+    }
+    public static AWS.Cryptography.DbEncryptionSDK.DynamoDb.GetEncryptedDataKeyDescriptionOutput FromDafny_N3_aws__N12_cryptography__N15_dbEncryptionSdk__N8_dynamoDb__S36_GetEncryptedDataKeyDescriptionOutput(software.amazon.cryptography.dbencryptionsdk.dynamodb.internaldafny.types._IGetEncryptedDataKeyDescriptionOutput value)
+    {
+      software.amazon.cryptography.dbencryptionsdk.dynamodb.internaldafny.types.GetEncryptedDataKeyDescriptionOutput concrete = (software.amazon.cryptography.dbencryptionsdk.dynamodb.internaldafny.types.GetEncryptedDataKeyDescriptionOutput)value; AWS.Cryptography.DbEncryptionSDK.DynamoDb.GetEncryptedDataKeyDescriptionOutput converted = new AWS.Cryptography.DbEncryptionSDK.DynamoDb.GetEncryptedDataKeyDescriptionOutput(); converted.EncryptedDataKeyDescriptionOutput = (System.Collections.Generic.List<AWS.Cryptography.DbEncryptionSDK.DynamoDb.EncryptedDataKeyDescription>)FromDafny_N3_aws__N12_cryptography__N15_dbEncryptionSdk__N8_dynamoDb__S36_GetEncryptedDataKeyDescriptionOutput__M33_EncryptedDataKeyDescriptionOutput(concrete._EncryptedDataKeyDescriptionOutput); return converted;
+    }
+    public static software.amazon.cryptography.dbencryptionsdk.dynamodb.internaldafny.types._IGetEncryptedDataKeyDescriptionOutput ToDafny_N3_aws__N12_cryptography__N15_dbEncryptionSdk__N8_dynamoDb__S36_GetEncryptedDataKeyDescriptionOutput(AWS.Cryptography.DbEncryptionSDK.DynamoDb.GetEncryptedDataKeyDescriptionOutput value)
+    {
+      value.Validate();
+
+      return new software.amazon.cryptography.dbencryptionsdk.dynamodb.internaldafny.types.GetEncryptedDataKeyDescriptionOutput(ToDafny_N3_aws__N12_cryptography__N15_dbEncryptionSdk__N8_dynamoDb__S36_GetEncryptedDataKeyDescriptionOutput__M33_EncryptedDataKeyDescriptionOutput(value.EncryptedDataKeyDescriptionOutput));
+    }
+    public static AWS.Cryptography.DbEncryptionSDK.DynamoDb.GetEncryptedDataKeyDescriptionUnion FromDafny_N3_aws__N12_cryptography__N15_dbEncryptionSdk__N8_dynamoDb__S35_GetEncryptedDataKeyDescriptionUnion(software.amazon.cryptography.dbencryptionsdk.dynamodb.internaldafny.types._IGetEncryptedDataKeyDescriptionUnion value)
+    {
+      software.amazon.cryptography.dbencryptionsdk.dynamodb.internaldafny.types.GetEncryptedDataKeyDescriptionUnion concrete = (software.amazon.cryptography.dbencryptionsdk.dynamodb.internaldafny.types.GetEncryptedDataKeyDescriptionUnion)value;
+      var converted = new AWS.Cryptography.DbEncryptionSDK.DynamoDb.GetEncryptedDataKeyDescriptionUnion(); if (value.is_header)
+      {
+        converted.Header = FromDafny_N3_aws__N12_cryptography__N15_dbEncryptionSdk__N8_dynamoDb__S35_GetEncryptedDataKeyDescriptionUnion__M6_header(concrete.dtor_header);
+        return converted;
+      }
+      if (value.is_item)
+      {
+        converted.Item = FromDafny_N3_aws__N12_cryptography__N15_dbEncryptionSdk__N8_dynamoDb__S35_GetEncryptedDataKeyDescriptionUnion__M4_item(concrete.dtor_item);
+        return converted;
+      }
+      throw new System.ArgumentException("Invalid AWS.Cryptography.DbEncryptionSDK.DynamoDb.GetEncryptedDataKeyDescriptionUnion state");
+    }
+    public static software.amazon.cryptography.dbencryptionsdk.dynamodb.internaldafny.types._IGetEncryptedDataKeyDescriptionUnion ToDafny_N3_aws__N12_cryptography__N15_dbEncryptionSdk__N8_dynamoDb__S35_GetEncryptedDataKeyDescriptionUnion(AWS.Cryptography.DbEncryptionSDK.DynamoDb.GetEncryptedDataKeyDescriptionUnion value)
+    {
+      value.Validate(); if (value.IsSetHeader())
+      {
+        return software.amazon.cryptography.dbencryptionsdk.dynamodb.internaldafny.types.GetEncryptedDataKeyDescriptionUnion.create_header(ToDafny_N3_aws__N12_cryptography__N15_dbEncryptionSdk__N8_dynamoDb__S35_GetEncryptedDataKeyDescriptionUnion__M6_header(value.Header));
+      }
+      if (value.IsSetItem())
+      {
+        return software.amazon.cryptography.dbencryptionsdk.dynamodb.internaldafny.types.GetEncryptedDataKeyDescriptionUnion.create_item(ToDafny_N3_aws__N12_cryptography__N15_dbEncryptionSdk__N8_dynamoDb__S35_GetEncryptedDataKeyDescriptionUnion__M4_item(value.Item));
+      }
+      throw new System.ArgumentException("Invalid AWS.Cryptography.DbEncryptionSDK.DynamoDb.GetEncryptedDataKeyDescriptionUnion state");
+    }
     public static AWS.Cryptography.DbEncryptionSDK.DynamoDb.LegacyPolicy FromDafny_N3_aws__N12_cryptography__N15_dbEncryptionSdk__N8_dynamoDb__S12_LegacyPolicy(software.amazon.cryptography.dbencryptionsdk.dynamodb.internaldafny.types._ILegacyPolicy value)
     {
       if (value.is_FORCE__LEGACY__ENCRYPT__ALLOW__LEGACY__DECRYPT) return AWS.Cryptography.DbEncryptionSDK.DynamoDb.LegacyPolicy.FORCE_LEGACY_ENCRYPT_ALLOW_LEGACY_DECRYPT;
@@ -376,6 +423,38 @@ namespace AWS.Cryptography.DbEncryptionSDK.DynamoDb
     {
       return ToDafny_N6_smithy__N3_api__S6_String(value);
     }
+    public static AWS.Cryptography.DbEncryptionSDK.DynamoDb.GetEncryptedDataKeyDescriptionUnion FromDafny_N3_aws__N12_cryptography__N15_dbEncryptionSdk__N8_dynamoDb__S35_GetEncryptedDataKeyDescriptionInput__M5_input(software.amazon.cryptography.dbencryptionsdk.dynamodb.internaldafny.types._IGetEncryptedDataKeyDescriptionUnion value)
+    {
+      return FromDafny_N3_aws__N12_cryptography__N15_dbEncryptionSdk__N8_dynamoDb__S35_GetEncryptedDataKeyDescriptionUnion(value);
+    }
+    public static software.amazon.cryptography.dbencryptionsdk.dynamodb.internaldafny.types._IGetEncryptedDataKeyDescriptionUnion ToDafny_N3_aws__N12_cryptography__N15_dbEncryptionSdk__N8_dynamoDb__S35_GetEncryptedDataKeyDescriptionInput__M5_input(AWS.Cryptography.DbEncryptionSDK.DynamoDb.GetEncryptedDataKeyDescriptionUnion value)
+    {
+      return ToDafny_N3_aws__N12_cryptography__N15_dbEncryptionSdk__N8_dynamoDb__S35_GetEncryptedDataKeyDescriptionUnion(value);
+    }
+    public static System.Collections.Generic.List<AWS.Cryptography.DbEncryptionSDK.DynamoDb.EncryptedDataKeyDescription> FromDafny_N3_aws__N12_cryptography__N15_dbEncryptionSdk__N8_dynamoDb__S36_GetEncryptedDataKeyDescriptionOutput__M33_EncryptedDataKeyDescriptionOutput(Dafny.ISequence<software.amazon.cryptography.dbencryptionsdk.dynamodb.internaldafny.types._IEncryptedDataKeyDescription> value)
+    {
+      return FromDafny_N3_aws__N12_cryptography__N15_dbEncryptionSdk__N8_dynamoDb__S31_EncryptedDataKeyDescriptionList(value);
+    }
+    public static Dafny.ISequence<software.amazon.cryptography.dbencryptionsdk.dynamodb.internaldafny.types._IEncryptedDataKeyDescription> ToDafny_N3_aws__N12_cryptography__N15_dbEncryptionSdk__N8_dynamoDb__S36_GetEncryptedDataKeyDescriptionOutput__M33_EncryptedDataKeyDescriptionOutput(System.Collections.Generic.List<AWS.Cryptography.DbEncryptionSDK.DynamoDb.EncryptedDataKeyDescription> value)
+    {
+      return ToDafny_N3_aws__N12_cryptography__N15_dbEncryptionSdk__N8_dynamoDb__S31_EncryptedDataKeyDescriptionList(value);
+    }
+    public static System.IO.MemoryStream FromDafny_N3_aws__N12_cryptography__N15_dbEncryptionSdk__N8_dynamoDb__S35_GetEncryptedDataKeyDescriptionUnion__M6_header(Dafny.ISequence<byte> value)
+    {
+      return FromDafny_N6_smithy__N3_api__S4_Blob(value);
+    }
+    public static Dafny.ISequence<byte> ToDafny_N3_aws__N12_cryptography__N15_dbEncryptionSdk__N8_dynamoDb__S35_GetEncryptedDataKeyDescriptionUnion__M6_header(System.IO.MemoryStream value)
+    {
+      return ToDafny_N6_smithy__N3_api__S4_Blob(value);
+    }
+    public static System.Collections.Generic.Dictionary<string, Amazon.DynamoDBv2.Model.AttributeValue> FromDafny_N3_aws__N12_cryptography__N15_dbEncryptionSdk__N8_dynamoDb__S35_GetEncryptedDataKeyDescriptionUnion__M4_item(Dafny.IMap<Dafny.ISequence<char>, software.amazon.cryptography.services.dynamodb.internaldafny.types._IAttributeValue> value)
+    {
+      return FromDafny_N3_com__N9_amazonaws__N8_dynamodb__S12_AttributeMap(value);
+    }
+    public static Dafny.IMap<Dafny.ISequence<char>, software.amazon.cryptography.services.dynamodb.internaldafny.types._IAttributeValue> ToDafny_N3_aws__N12_cryptography__N15_dbEncryptionSdk__N8_dynamoDb__S35_GetEncryptedDataKeyDescriptionUnion__M4_item(System.Collections.Generic.Dictionary<string, Amazon.DynamoDBv2.Model.AttributeValue> value)
+    {
+      return ToDafny_N3_com__N9_amazonaws__N8_dynamodb__S12_AttributeMap(value);
+    }
     public static AWS.Cryptography.DbEncryptionSDK.DynamoDb.Upper FromDafny_N3_aws__N12_cryptography__N15_dbEncryptionSdk__N8_dynamoDb__S16_VirtualTransform__M5_upper(software.amazon.cryptography.dbencryptionsdk.dynamodb.internaldafny.types._IUpper value)
     {
       return FromDafny_N3_aws__N12_cryptography__N15_dbEncryptionSdk__N8_dynamoDb__S5_Upper(value);
@@ -552,6 +631,37 @@ namespace AWS.Cryptography.DbEncryptionSDK.DynamoDb
          new Dafny.Pair<Dafny.ISequence<char>, software.amazon.cryptography.services.dynamodb.internaldafny.types._IAttributeValue>(ToDafny_N3_com__N9_amazonaws__N8_dynamodb__S3_Key__M3_key(pair.Key), ToDafny_N3_com__N9_amazonaws__N8_dynamodb__S3_Key__M5_value(pair.Value))
      ));
     }
+    public static System.Collections.Generic.List<AWS.Cryptography.DbEncryptionSDK.DynamoDb.EncryptedDataKeyDescription> FromDafny_N3_aws__N12_cryptography__N15_dbEncryptionSdk__N8_dynamoDb__S31_EncryptedDataKeyDescriptionList(Dafny.ISequence<software.amazon.cryptography.dbencryptionsdk.dynamodb.internaldafny.types._IEncryptedDataKeyDescription> value)
+    {
+      return new System.Collections.Generic.List<AWS.Cryptography.DbEncryptionSDK.DynamoDb.EncryptedDataKeyDescription>(value.Elements.Select(FromDafny_N3_aws__N12_cryptography__N15_dbEncryptionSdk__N8_dynamoDb__S31_EncryptedDataKeyDescriptionList__M6_member));
+    }
+    public static Dafny.ISequence<software.amazon.cryptography.dbencryptionsdk.dynamodb.internaldafny.types._IEncryptedDataKeyDescription> ToDafny_N3_aws__N12_cryptography__N15_dbEncryptionSdk__N8_dynamoDb__S31_EncryptedDataKeyDescriptionList(System.Collections.Generic.List<AWS.Cryptography.DbEncryptionSDK.DynamoDb.EncryptedDataKeyDescription> value)
+    {
+      return Dafny.Sequence<software.amazon.cryptography.dbencryptionsdk.dynamodb.internaldafny.types._IEncryptedDataKeyDescription>.FromArray(value.Select(ToDafny_N3_aws__N12_cryptography__N15_dbEncryptionSdk__N8_dynamoDb__S31_EncryptedDataKeyDescriptionList__M6_member).ToArray());
+    }
+    public static System.IO.MemoryStream FromDafny_N6_smithy__N3_api__S4_Blob(Dafny.ISequence<byte> value)
+    {
+      return new System.IO.MemoryStream(value.Elements);
+    }
+    public static Dafny.ISequence<byte> ToDafny_N6_smithy__N3_api__S4_Blob(System.IO.MemoryStream value)
+    {
+      if (value.ToArray().Length == 0 && value.Length > 0)
+      {
+        throw new System.ArgumentException("Fatal Error: MemoryStream instance not backed by an array!");
+      }
+      return Dafny.Sequence<byte>.FromArray(value.ToArray());
+
+    }
+    public static System.Collections.Generic.Dictionary<string, Amazon.DynamoDBv2.Model.AttributeValue> FromDafny_N3_com__N9_amazonaws__N8_dynamodb__S12_AttributeMap(Dafny.IMap<Dafny.ISequence<char>, software.amazon.cryptography.services.dynamodb.internaldafny.types._IAttributeValue> value)
+    {
+      return value.ItemEnumerable.ToDictionary(pair => FromDafny_N3_com__N9_amazonaws__N8_dynamodb__S12_AttributeMap__M3_key(pair.Car), pair => FromDafny_N3_com__N9_amazonaws__N8_dynamodb__S12_AttributeMap__M5_value(pair.Cdr));
+    }
+    public static Dafny.IMap<Dafny.ISequence<char>, software.amazon.cryptography.services.dynamodb.internaldafny.types._IAttributeValue> ToDafny_N3_com__N9_amazonaws__N8_dynamodb__S12_AttributeMap(System.Collections.Generic.Dictionary<string, Amazon.DynamoDBv2.Model.AttributeValue> value)
+    {
+      return Dafny.Map<Dafny.ISequence<char>, software.amazon.cryptography.services.dynamodb.internaldafny.types._IAttributeValue>.FromCollection(value.Select(pair =>
+         new Dafny.Pair<Dafny.ISequence<char>, software.amazon.cryptography.services.dynamodb.internaldafny.types._IAttributeValue>(ToDafny_N3_com__N9_amazonaws__N8_dynamodb__S12_AttributeMap__M3_key(pair.Key), ToDafny_N3_com__N9_amazonaws__N8_dynamodb__S12_AttributeMap__M5_value(pair.Value))
+     ));
+    }
     public static AWS.Cryptography.DbEncryptionSDK.DynamoDb.Upper FromDafny_N3_aws__N12_cryptography__N15_dbEncryptionSdk__N8_dynamoDb__S5_Upper(software.amazon.cryptography.dbencryptionsdk.dynamodb.internaldafny.types._IUpper value)
     {
       software.amazon.cryptography.dbencryptionsdk.dynamodb.internaldafny.types.Upper concrete = (software.amazon.cryptography.dbencryptionsdk.dynamodb.internaldafny.types.Upper)value; AWS.Cryptography.DbEncryptionSDK.DynamoDb.Upper converted = new AWS.Cryptography.DbEncryptionSDK.DynamoDb.Upper(); return converted;
@@ -705,6 +815,30 @@ namespace AWS.Cryptography.DbEncryptionSDK.DynamoDb
       return FromDafny_N3_com__N9_amazonaws__N8_dynamodb__S14_AttributeValue(value);
     }
     public static software.amazon.cryptography.services.dynamodb.internaldafny.types._IAttributeValue ToDafny_N3_com__N9_amazonaws__N8_dynamodb__S3_Key__M5_value(Amazon.DynamoDBv2.Model.AttributeValue value)
+    {
+      return ToDafny_N3_com__N9_amazonaws__N8_dynamodb__S14_AttributeValue(value);
+    }
+    public static AWS.Cryptography.DbEncryptionSDK.DynamoDb.EncryptedDataKeyDescription FromDafny_N3_aws__N12_cryptography__N15_dbEncryptionSdk__N8_dynamoDb__S31_EncryptedDataKeyDescriptionList__M6_member(software.amazon.cryptography.dbencryptionsdk.dynamodb.internaldafny.types._IEncryptedDataKeyDescription value)
+    {
+      return FromDafny_N3_aws__N12_cryptography__N15_dbEncryptionSdk__N8_dynamoDb__S27_EncryptedDataKeyDescription(value);
+    }
+    public static software.amazon.cryptography.dbencryptionsdk.dynamodb.internaldafny.types._IEncryptedDataKeyDescription ToDafny_N3_aws__N12_cryptography__N15_dbEncryptionSdk__N8_dynamoDb__S31_EncryptedDataKeyDescriptionList__M6_member(AWS.Cryptography.DbEncryptionSDK.DynamoDb.EncryptedDataKeyDescription value)
+    {
+      return ToDafny_N3_aws__N12_cryptography__N15_dbEncryptionSdk__N8_dynamoDb__S27_EncryptedDataKeyDescription(value);
+    }
+    public static string FromDafny_N3_com__N9_amazonaws__N8_dynamodb__S12_AttributeMap__M3_key(Dafny.ISequence<char> value)
+    {
+      return FromDafny_N3_com__N9_amazonaws__N8_dynamodb__S13_AttributeName(value);
+    }
+    public static Dafny.ISequence<char> ToDafny_N3_com__N9_amazonaws__N8_dynamodb__S12_AttributeMap__M3_key(string value)
+    {
+      return ToDafny_N3_com__N9_amazonaws__N8_dynamodb__S13_AttributeName(value);
+    }
+    public static Amazon.DynamoDBv2.Model.AttributeValue FromDafny_N3_com__N9_amazonaws__N8_dynamodb__S12_AttributeMap__M5_value(software.amazon.cryptography.services.dynamodb.internaldafny.types._IAttributeValue value)
+    {
+      return FromDafny_N3_com__N9_amazonaws__N8_dynamodb__S14_AttributeValue(value);
+    }
+    public static software.amazon.cryptography.services.dynamodb.internaldafny.types._IAttributeValue ToDafny_N3_com__N9_amazonaws__N8_dynamodb__S12_AttributeMap__M5_value(Amazon.DynamoDBv2.Model.AttributeValue value)
     {
       return ToDafny_N3_com__N9_amazonaws__N8_dynamodb__S14_AttributeValue(value);
     }
@@ -957,6 +1091,21 @@ namespace AWS.Cryptography.DbEncryptionSDK.DynamoDb
       }
       throw new System.ArgumentException("Invalid Amazon.DynamoDBv2.Model.AttributeValue state");
     }
+    public static AWS.Cryptography.DbEncryptionSDK.DynamoDb.EncryptedDataKeyDescription FromDafny_N3_aws__N12_cryptography__N15_dbEncryptionSdk__N8_dynamoDb__S27_EncryptedDataKeyDescription(software.amazon.cryptography.dbencryptionsdk.dynamodb.internaldafny.types._IEncryptedDataKeyDescription value)
+    {
+      software.amazon.cryptography.dbencryptionsdk.dynamodb.internaldafny.types.EncryptedDataKeyDescription concrete = (software.amazon.cryptography.dbencryptionsdk.dynamodb.internaldafny.types.EncryptedDataKeyDescription)value; AWS.Cryptography.DbEncryptionSDK.DynamoDb.EncryptedDataKeyDescription converted = new AWS.Cryptography.DbEncryptionSDK.DynamoDb.EncryptedDataKeyDescription(); converted.KeyProviderId = (string)FromDafny_N3_aws__N12_cryptography__N15_dbEncryptionSdk__N8_dynamoDb__S27_EncryptedDataKeyDescription__M13_keyProviderId(concrete._keyProviderId);
+      if (concrete._keyProviderInfo.is_Some) converted.KeyProviderInfo = (string)FromDafny_N3_aws__N12_cryptography__N15_dbEncryptionSdk__N8_dynamoDb__S27_EncryptedDataKeyDescription__M15_keyProviderInfo(concrete._keyProviderInfo);
+      if (concrete._branchKeyId.is_Some) converted.BranchKeyId = (string)FromDafny_N3_aws__N12_cryptography__N15_dbEncryptionSdk__N8_dynamoDb__S27_EncryptedDataKeyDescription__M11_branchKeyId(concrete._branchKeyId);
+      if (concrete._branchKeyVersion.is_Some) converted.BranchKeyVersion = (string)FromDafny_N3_aws__N12_cryptography__N15_dbEncryptionSdk__N8_dynamoDb__S27_EncryptedDataKeyDescription__M16_branchKeyVersion(concrete._branchKeyVersion); return converted;
+    }
+    public static software.amazon.cryptography.dbencryptionsdk.dynamodb.internaldafny.types._IEncryptedDataKeyDescription ToDafny_N3_aws__N12_cryptography__N15_dbEncryptionSdk__N8_dynamoDb__S27_EncryptedDataKeyDescription(AWS.Cryptography.DbEncryptionSDK.DynamoDb.EncryptedDataKeyDescription value)
+    {
+      value.Validate();
+      string var_keyProviderInfo = value.IsSetKeyProviderInfo() ? value.KeyProviderInfo : (string)null;
+      string var_branchKeyId = value.IsSetBranchKeyId() ? value.BranchKeyId : (string)null;
+      string var_branchKeyVersion = value.IsSetBranchKeyVersion() ? value.BranchKeyVersion : (string)null;
+      return new software.amazon.cryptography.dbencryptionsdk.dynamodb.internaldafny.types.EncryptedDataKeyDescription(ToDafny_N3_aws__N12_cryptography__N15_dbEncryptionSdk__N8_dynamoDb__S27_EncryptedDataKeyDescription__M13_keyProviderId(value.KeyProviderId), ToDafny_N3_aws__N12_cryptography__N15_dbEncryptionSdk__N8_dynamoDb__S27_EncryptedDataKeyDescription__M15_keyProviderInfo(var_keyProviderInfo), ToDafny_N3_aws__N12_cryptography__N15_dbEncryptionSdk__N8_dynamoDb__S27_EncryptedDataKeyDescription__M11_branchKeyId(var_branchKeyId), ToDafny_N3_aws__N12_cryptography__N15_dbEncryptionSdk__N8_dynamoDb__S27_EncryptedDataKeyDescription__M16_branchKeyVersion(var_branchKeyVersion));
+    }
     public static string FromDafny_N3_aws__N12_cryptography__N15_dbEncryptionSdk__N8_dynamoDb__S4_Char(Dafny.ISequence<char> value)
     {
       return new string(value.Elements);
@@ -1084,6 +1233,38 @@ namespace AWS.Cryptography.DbEncryptionSDK.DynamoDb
     public static bool ToDafny_N3_com__N9_amazonaws__N8_dynamodb__S14_AttributeValue__M4_BOOL(bool value)
     {
       return ToDafny_N3_com__N9_amazonaws__N8_dynamodb__S21_BooleanAttributeValue(value);
+    }
+    public static string FromDafny_N3_aws__N12_cryptography__N15_dbEncryptionSdk__N8_dynamoDb__S27_EncryptedDataKeyDescription__M13_keyProviderId(Dafny.ISequence<char> value)
+    {
+      return FromDafny_N6_smithy__N3_api__S6_String(value);
+    }
+    public static Dafny.ISequence<char> ToDafny_N3_aws__N12_cryptography__N15_dbEncryptionSdk__N8_dynamoDb__S27_EncryptedDataKeyDescription__M13_keyProviderId(string value)
+    {
+      return ToDafny_N6_smithy__N3_api__S6_String(value);
+    }
+    public static string FromDafny_N3_aws__N12_cryptography__N15_dbEncryptionSdk__N8_dynamoDb__S27_EncryptedDataKeyDescription__M15_keyProviderInfo(Wrappers_Compile._IOption<Dafny.ISequence<char>> value)
+    {
+      return value.is_None ? (string)null : FromDafny_N6_smithy__N3_api__S6_String(value.Extract());
+    }
+    public static Wrappers_Compile._IOption<Dafny.ISequence<char>> ToDafny_N3_aws__N12_cryptography__N15_dbEncryptionSdk__N8_dynamoDb__S27_EncryptedDataKeyDescription__M15_keyProviderInfo(string value)
+    {
+      return value == null ? Wrappers_Compile.Option<Dafny.ISequence<char>>.create_None() : Wrappers_Compile.Option<Dafny.ISequence<char>>.create_Some(ToDafny_N6_smithy__N3_api__S6_String((string)value));
+    }
+    public static string FromDafny_N3_aws__N12_cryptography__N15_dbEncryptionSdk__N8_dynamoDb__S27_EncryptedDataKeyDescription__M11_branchKeyId(Wrappers_Compile._IOption<Dafny.ISequence<char>> value)
+    {
+      return value.is_None ? (string)null : FromDafny_N6_smithy__N3_api__S6_String(value.Extract());
+    }
+    public static Wrappers_Compile._IOption<Dafny.ISequence<char>> ToDafny_N3_aws__N12_cryptography__N15_dbEncryptionSdk__N8_dynamoDb__S27_EncryptedDataKeyDescription__M11_branchKeyId(string value)
+    {
+      return value == null ? Wrappers_Compile.Option<Dafny.ISequence<char>>.create_None() : Wrappers_Compile.Option<Dafny.ISequence<char>>.create_Some(ToDafny_N6_smithy__N3_api__S6_String((string)value));
+    }
+    public static string FromDafny_N3_aws__N12_cryptography__N15_dbEncryptionSdk__N8_dynamoDb__S27_EncryptedDataKeyDescription__M16_branchKeyVersion(Wrappers_Compile._IOption<Dafny.ISequence<char>> value)
+    {
+      return value.is_None ? (string)null : FromDafny_N6_smithy__N3_api__S6_String(value.Extract());
+    }
+    public static Wrappers_Compile._IOption<Dafny.ISequence<char>> ToDafny_N3_aws__N12_cryptography__N15_dbEncryptionSdk__N8_dynamoDb__S27_EncryptedDataKeyDescription__M16_branchKeyVersion(string value)
+    {
+      return value == null ? Wrappers_Compile.Option<Dafny.ISequence<char>>.create_None() : Wrappers_Compile.Option<Dafny.ISequence<char>>.create_Some(ToDafny_N6_smithy__N3_api__S6_String((string)value));
     }
     public static AWS.Cryptography.MaterialProviders.DefaultCache FromDafny_N3_aws__N12_cryptography__N17_materialProviders__S12_DefaultCache(software.amazon.cryptography.materialproviders.internaldafny.types._IDefaultCache value)
     {
