Examples/runtimes/java/DynamoDbEncryption/src/test/java/software/amazon/cryptography/examples/TestGetEncryptedDataKeyDescriptionExample.java
@@ -1,0 +1,10 @@
+package software.amazon.cryptography.examples;
+
+import org.testng.annotations.Test;
+
+public class TestGetEncryptedDataKeyDescriptionExample {
+    @Test
+    public void TestGetEncryptedDataKeyDescription() {
+        GetEncryptedDataKeyDescriptionExample.getEncryptedDataKeyDescription(TestUtils.TEST_DDB_TABLE_NAME,"partition_key","BasicPutGetExample","sort_key","0","aws-kms",TestUtils.TEST_KMS_KEY_ID,null,null);
+    }
+}
