DynamoDbEncryption/dafny/DynamoDbEncryption/Model/AwsCryptographyDbEncryptionSdkDynamoDbTypes.dfy
@@ -91,8 +91,10 @@ module {:extern "software.amazon.cryptography.dbencryptionsdk.dynamodb.internald
   class IDynamoDbEncryptionClientCallHistory {
     ghost constructor() {
       CreateDynamoDbEncryptionBranchKeyIdSupplier := [];
+      GetEncryptedDataKeyDescription := [];
     }
     ghost var CreateDynamoDbEncryptionBranchKeyIdSupplier: seq<DafnyCallEvent<CreateDynamoDbEncryptionBranchKeyIdSupplierInput, Result<CreateDynamoDbEncryptionBranchKeyIdSupplierOutput, Error>>>
+    ghost var GetEncryptedDataKeyDescription: seq<DafnyCallEvent<GetEncryptedDataKeyDescriptionInput, Result<GetEncryptedDataKeyDescriptionOutput, Error>>>
   }
   trait {:termination false} IDynamoDbEncryptionClient
   {
@@ -144,6 +146,21 @@ module {:extern "software.amazon.cryptography.dbencryptionsdk.dynamodb.internald
                && fresh ( output.value.branchKeyIdSupplier.Modifies - Modifies - {History} - input.ddbKeyBranchKeyIdSupplier.Modifies ) )
       ensures CreateDynamoDbEncryptionBranchKeyIdSupplierEnsuresPublicly(input, output)
       ensures History.CreateDynamoDbEncryptionBranchKeyIdSupplier == old(History.CreateDynamoDbEncryptionBranchKeyIdSupplier) + [DafnyCallEvent(input, output)]
+
+    predicate GetEncryptedDataKeyDescriptionEnsuresPublicly(input: GetEncryptedDataKeyDescriptionInput , output: Result<GetEncryptedDataKeyDescriptionOutput, Error>)
+    // The public method to be called by library consumers
+    method GetEncryptedDataKeyDescription ( input: GetEncryptedDataKeyDescriptionInput )
+      returns (output: Result<GetEncryptedDataKeyDescriptionOutput, Error>)
+      requires
+        && ValidState()
+      modifies Modifies - {History} ,
+               History`GetEncryptedDataKeyDescription
+      // Dafny will skip type parameters when generating a default decreases clause.
+      decreases Modifies - {History}
+      ensures
+        && ValidState()
+      ensures GetEncryptedDataKeyDescriptionEnsuresPublicly(input, output)
+      ensures History.GetEncryptedDataKeyDescription == old(History.GetEncryptedDataKeyDescription) + [DafnyCallEvent(input, output)]
 
   }
   datatype DynamoDbEncryptionConfig = | DynamoDbEncryptionConfig (
@@ -232,6 +249,13 @@ module {:extern "software.amazon.cryptography.dbencryptionsdk.dynamodb.internald
   datatype DynamoDbTablesEncryptionConfig = | DynamoDbTablesEncryptionConfig (
     nameonly tableEncryptionConfigs: DynamoDbTableEncryptionConfigList
   )
+  datatype EncryptedDataKeyDescription = | EncryptedDataKeyDescription (
+    nameonly keyProviderId: string ,
+    nameonly keyProviderInfo: Option<string> := Option.None ,
+    nameonly branchKeyId: Option<string> := Option.None ,
+    nameonly branchKeyVersion: Option<string> := Option.None
+  )
+  type EncryptedDataKeyDescriptionList = seq<EncryptedDataKeyDescription>
   datatype EncryptedPart = | EncryptedPart (
     nameonly name: string ,
     nameonly prefix: Prefix
@@ -246,6 +270,15 @@ module {:extern "software.amazon.cryptography.dbencryptionsdk.dynamodb.internald
   datatype GetBranchKeyIdFromDdbKeyOutput = | GetBranchKeyIdFromDdbKeyOutput (
     nameonly branchKeyId: string
   )
+  datatype GetEncryptedDataKeyDescriptionInput = | GetEncryptedDataKeyDescriptionInput (
+    nameonly input: GetEncryptedDataKeyDescriptionUnion
+  )
+  datatype GetEncryptedDataKeyDescriptionOutput = | GetEncryptedDataKeyDescriptionOutput (
+    nameonly EncryptedDataKeyDescriptionOutput: EncryptedDataKeyDescriptionList
+  )
+  datatype GetEncryptedDataKeyDescriptionUnion =
+    | header(header: seq<uint8>)
+    | item(item: ComAmazonawsDynamodbTypes.AttributeMap)
   datatype GetPrefix = | GetPrefix (
     nameonly length: int32
   )
@@ -510,6 +543,26 @@ abstract module AbstractAwsCryptographyDbEncryptionSdkDynamoDbService
       History.CreateDynamoDbEncryptionBranchKeyIdSupplier := History.CreateDynamoDbEncryptionBranchKeyIdSupplier + [DafnyCallEvent(input, output)];
     }
 
+    predicate GetEncryptedDataKeyDescriptionEnsuresPublicly(input: GetEncryptedDataKeyDescriptionInput , output: Result<GetEncryptedDataKeyDescriptionOutput, Error>)
+    {Operations.GetEncryptedDataKeyDescriptionEnsuresPublicly(input, output)}
+    // The public method to be called by library consumers
+    method GetEncryptedDataKeyDescription ( input: GetEncryptedDataKeyDescriptionInput )
+      returns (output: Result<GetEncryptedDataKeyDescriptionOutput, Error>)
+      requires
+        && ValidState()
+      modifies Modifies - {History} ,
+               History`GetEncryptedDataKeyDescription
+      // Dafny will skip type parameters when generating a default decreases clause.
+      decreases Modifies - {History}
+      ensures
+        && ValidState()
+      ensures GetEncryptedDataKeyDescriptionEnsuresPublicly(input, output)
+      ensures History.GetEncryptedDataKeyDescription == old(History.GetEncryptedDataKeyDescription) + [DafnyCallEvent(input, output)]
+    {
+      output := Operations.GetEncryptedDataKeyDescription(config, input);
+      History.GetEncryptedDataKeyDescription := History.GetEncryptedDataKeyDescription + [DafnyCallEvent(input, output)];
+    }
+
   }
 }
 abstract module AbstractAwsCryptographyDbEncryptionSdkDynamoDbOperations {
@@ -541,4 +594,20 @@ abstract module AbstractAwsCryptographyDbEncryptionSdkDynamoDbOperations {
              && fresh(output.value.branchKeyIdSupplier)
              && fresh ( output.value.branchKeyIdSupplier.Modifies - ModifiesInternalConfig(config) - input.ddbKeyBranchKeyIdSupplier.Modifies ) )
     ensures CreateDynamoDbEncryptionBranchKeyIdSupplierEnsuresPublicly(input, output)
+
+
+  predicate GetEncryptedDataKeyDescriptionEnsuresPublicly(input: GetEncryptedDataKeyDescriptionInput , output: Result<GetEncryptedDataKeyDescriptionOutput, Error>)
+  // The private method to be refined by the library developer
+
+
+  method GetEncryptedDataKeyDescription ( config: InternalConfig , input: GetEncryptedDataKeyDescriptionInput )
+    returns (output: Result<GetEncryptedDataKeyDescriptionOutput, Error>)
+    requires
+      && ValidInternalConfig?(config)
+    modifies ModifiesInternalConfig(config)
+    // Dafny will skip type parameters when generating a default decreases clause.
+    decreases ModifiesInternalConfig(config)
+    ensures
+      && ValidInternalConfig?(config)
+    ensures GetEncryptedDataKeyDescriptionEnsuresPublicly(input, output)
 }
